src/lang/Local.v
@@ -261,30 +261,14 @@ Module Local.
   .
   Hint Constructors write_step.
 
-  Inductive write_na_messages (ts: Time.t)
-                              (promises1 mem1: Memory.t) (loc: Loc.t) (from to: Time.t) (val: Const.t)
-                              (promises2 mem2: Memory.t) (kind: Memory.op_kind): Prop :=
-  | write_na_messages_base
-      (WRITABLE: Time.lt ts to)
-      (WRITE: Memory.write promises1 mem1 loc from to (Message.concrete val None) promises2 mem2 kind)
-  | write_na_messages_write
-      from' to' msg' promises' mem' kind'
-      (WRITABLE_EX: Time.lt ts to')
-      (MSG_EX: __guard__ (msg' = Message.undef \/
-                          exists val', msg' = Message.concrete val' None))
-      (WRITE_EX: Memory.write promises1 mem1 loc from' to' msg' promises' mem' kind')
-      (WRITE_NA: write_na_messages to' promises' mem' loc from to val promises2 mem2 kind)
-  .
-  Hint Constructors write_na_messages.
-
   Inductive write_na_step (lc1:t) (sc1:TimeMap.t) (mem1:Memory.t)
                           (loc:Loc.t) (from to:Time.t) (val:Const.t) (ord:Ordering.t)
                           (lc2:t) (sc2:TimeMap.t) (mem2:Memory.t) (kind:Memory.op_kind): Prop :=
   | write_na_step_intro
       promises2
       (ORD: Ordering.le ord Ordering.na)
-      (WRITE: write_na_messages (View.rlx (TView.cur (tview lc1)) loc)
-                                (promises lc1) mem1 loc from to val promises2 mem2 kind)
+      (WRITE: Memory.write_na (View.rlx (TView.cur (tview lc1)) loc)
+                              (promises lc1) mem1 loc from to val promises2 mem2 kind)
       (LC2: lc2 = mk (TView.write_tview (tview lc1) sc1 loc to ord) promises2)
       (SC2: sc2 = sc1)
   .
@@ -491,11 +475,11 @@ Module Local.
     - inv WRITE. inv PROMISE; try inv TS; ss.
   Qed.
 
-  Lemma write_na_messages_future
+  Lemma write_na_future
         tview sc ord
         ts promises1 mem1 loc from to val promises2 mem2 kind
         (ORD: Ordering.le ord Ordering.na)
-        (WRITE: write_na_messages ts promises1 mem1 loc from to val promises2 mem2 kind)
+        (WRITE: Memory.write_na ts promises1 mem1 loc from to val promises2 mem2 kind)
         (WF_TVIEW1: TView.wf tview)
         (CLOSED_TVIEW1: TView.closed tview mem1)
         (CLOSED_SC1: Memory.closed_timemap sc mem1)
@@ -546,7 +530,7 @@ Module Local.
     <<MEM_FUTURE: Memory.future mem1 mem2>>.
   Proof.
     inv WF1. inv STEP.
-    exploit write_na_messages_future; eauto. i. des.
+    exploit write_na_future; eauto. i. des.
     splits; eauto; try refl.
     - eauto using Memory.future_closed_timemap.
     - apply TViewFacts.write_tview_incr. ss.
@@ -635,15 +619,6 @@ Module Local.
     inv STEP. eauto using Memory.promise_inhabited.
   Qed.
 
-  Lemma write_na_messages_inhabited
-        ts promises1 mem1 loc from to val promises2 mem2 kind
-        (WRITE: write_na_messages ts promises1 mem1 loc from to val promises2 mem2 kind)
-        (INHABITED1: Memory.inhabited mem1):
-    <<INHABITED2: Memory.inhabited mem2>>.
-  Proof.
-    induction WRITE; eauto using Memory.write_inhabited.
-  Qed.
-
   Lemma program_step_inhabited
         e lc1 sc1 mem1 lc2 sc2 mem2
         (STEP: program_step e lc1 sc1 mem1 lc2 sc2 mem2)
@@ -653,7 +628,7 @@ Module Local.
     inv STEP; eauto.
     - inv LOCAL. eauto using Memory.write_inhabited.
     - inv LOCAL2. eauto using Memory.write_inhabited.
-    - inv LOCAL. eauto using write_na_messages_inhabited.
+    - inv LOCAL. eauto using Memory.write_na_inhabited.
   Qed.
 
 
@@ -705,25 +680,6 @@ Module Local.
     inv WRITE. eapply TView.promise_closed; eauto.
   Qed.
 
-  Lemma write_na_messages_disjoint
-        ts promises1 mem1 loc from to val promises2 mem2 kind promises
-        (WRITE: write_na_messages ts promises1 mem1 loc from to val promises2 mem2 kind)
-        (LE1: Memory.le promises1 mem1)
-        (FINITE1: Memory.finite promises1)
-        (BOT1: Memory.bot_none promises1)
-        (CLOSED1: Memory.closed mem1)
-        (DISJOINT1: Memory.disjoint promises1 promises)
-        (LE: Memory.le promises mem1):
-    (<<DISJOINT2: Memory.disjoint promises2 promises>>) /\
-    (<<LE: Memory.le promises mem2>>).
-  Proof.
-    induction WRITE.
-    { exploit Memory.write_disjoint; try exact WRITE; eauto. }
-    exploit Memory.write_future; try exact WRITE_EX; eauto.
-    { unguard. des; subst; eauto. }
-    exploit Memory.write_disjoint; try exact WRITE_EX; eauto. i. des. eauto.
-  Qed.
-
   Lemma write_na_step_disjoint
         lc1 sc1 mem1 loc from to val ord lc2 sc2 mem2 kind lc
         (STEP: write_na_step lc1 sc1 mem1 loc from to val ord lc2 sc2 mem2 kind)
@@ -737,7 +693,7 @@ Module Local.
   Proof.
     exploit write_na_step_future; eauto. i. des.
     inv WF1. inv DISJOINT1. inversion WF. inv STEP.
-    exploit write_na_messages_disjoint; try apply WRITE; eauto. i. des.
+    exploit Memory.write_na_disjoint; try apply WRITE; eauto. i. des.
     splits; ss. econs; eauto.
     eapply TView.future_closed; eauto.
   Qed.
@@ -785,15 +741,6 @@ Module Local.
     - exploit write_na_step_disjoint; eauto.
   Qed.
 
-  Lemma write_na_messages_promises_bot
-        ts promises1 mem1 loc from to val promises2 mem2 kind
-        (WRITE: write_na_messages ts promises1 mem1 loc from to val promises2 mem2 kind)
-        (PROMISES1: promises1 = Memory.bot):
-    <<PROMISES2: promises2 = Memory.bot>>.
-  Proof.
-    induction WRITE; eauto using Memory.write_promises_bot.
-  Qed.
-
   Lemma program_step_promises_bot
         e lc1 sc1 mem1 lc2 sc2 mem2
         (STEP: program_step e lc1 sc1 mem1 lc2 sc2 mem2)
@@ -804,31 +751,7 @@ Module Local.
     - eapply Memory.write_promises_bot; eauto.
     - inv LOCAL1. inv LOCAL2.
       eapply Memory.write_promises_bot; eauto.
-    - eapply write_na_messages_promises_bot; eauto.
-  Qed.
-
-  Lemma write_na_messages_get_diff_promise
-        ts promises1 mem1 loc from to val promises2 mem2 kind
-        loc'
-        (WRITE: write_na_messages ts promises1 mem1 loc from to val promises2 mem2 kind)
-        (LOC: loc' <> loc):
-    forall to', Memory.get loc' to' promises2 = Memory.get loc' to' promises1.
-  Proof.
-    induction WRITE; eauto using Memory.write_get_diff_promise.
-    i. rewrite IHWRITE; eauto.
-    eapply Memory.write_get_diff_promise; eauto.
-  Qed.
-
-  Lemma write_na_messages_get_diff
-        ts promises1 mem1 loc from to val promises2 mem2 kind
-        loc'
-        (WRITE: write_na_messages ts promises1 mem1 loc from to val promises2 mem2 kind)
-        (LOC: loc' <> loc):
-    forall to', Memory.get loc' to' mem2 = Memory.get loc' to' mem1.
-  Proof.
-    induction WRITE; eauto using Memory.write_get_diff.
-    i. rewrite IHWRITE; eauto.
-    eapply Memory.write_get_diff; eauto.
+    - eapply Memory.write_na_promises_bot; eauto.
   Qed.
 
   Lemma program_step_get_diff_promises
@@ -844,7 +767,7 @@ Module Local.
     - i. inv LOCAL1. inv LOCAL2. s.
       erewrite <- Memory.write_get_diff_promise; eauto.
     - i. inv LOCAL.
-      erewrite <- write_na_messages_get_diff_promise; eauto.
+      erewrite <- Memory.write_na_get_diff_promise; eauto.
   Qed.
 
   Lemma program_step_get_diff
@@ -860,6 +783,6 @@ Module Local.
     - i. inv LOCAL1. inv LOCAL2. s.
       erewrite <- Memory.write_get_diff; eauto.
     - i. inv LOCAL.
-      erewrite <- write_na_messages_get_diff; try exact WRITE; eauto.
+      erewrite <- Memory.write_na_get_diff; try exact WRITE; eauto.
   Qed.
 End Local.
